glue/riscv/falcon/normalization_lemmas.i.dfy
@@ -1,50 +1,24 @@
 include "bv32_falcon_lemmas.i.dfy"
 include "mq_arith_lemmas.dfy"
-include "../bv16_op_s.dfy"
 
 module normalization_lemmas {
     import opened bv32_falcon_lemmas
     import opened mem
     import opened rv_machine
     import opened integers
-    import opened ntt_512_params
+    import opened falcon_512_i
     import opened bv32_op_s
     import opened mq_arith_lemmas
 
     import bv16_op_s
 
     const Q_HLAF :int := Q/2
-
-    predicate int_is_normalized(e: int)
-    {
-        -Q_HLAF <= e <= Q_HLAF
-    }
-
-    type nelem = e: int | int_is_normalized(e)
-
-    // 0 <= e < Q -> -Q/2 <= e <= Q/2
-    function normalize(e: elem): nelem
-    {
-        if e <= Q_HLAF then e else e as int - Q
-    }
-
-    // -Q/2 <= e < Q/2 -> 0 <= e <= Q 
-    function denormalize(e: nelem): elem
-    {
-        if e >= 0 then e else e + Q
-    }
-
-    lemma normalize_inverse(e: elem)
-        ensures denormalize(normalize(e)) == e;
-    {}
-
-    lemma denormalize_inverse(e: nelem)
-        ensures normalize(denormalize(e)) == e;
-    {}
+    const Q := falcon_512_i.Q;
+    const N := falcon_512_i.N;
 
     predicate uint16_is_normalized(e: uint16)
     {
-        int_is_normalized(bv16_op_s.to_int16(e))
+        MQN.int_is_normalized(bv16_op_s.to_int16(e))
     }
 
     // bascially convert to int16, but with requires
@@ -63,7 +37,7 @@ module normalization_lemmas {
         && (forall i | 0 <= i < |a| :: uint16_is_normalized(a[i]))
     }
 
-    function uint16_buff_as_n_elems(a: seq<uint16>): (na: seq<nelem>)
+    function uint16_buff_as_n_nelems(a: seq<uint16>): (na: seq<nelem>)
         requires normalized_values(a);
     {
         reveal normalized_values();
@@ -85,7 +59,7 @@ module normalization_lemmas {
         requires c == uint32_and(b, Q);
         requires d == uint32_add(a1, c);
         ensures uint16_is_normalized(buff[i]);
-        ensures d == denormalize(uint16_as_nelem(buff[i]));
+        ensures d == MQN.denormalize(uint16_as_nelem(buff[i]));
     {
         assert uint16_is_normalized(buff[i]) by {
             reveal normalized_values();
@@ -102,7 +76,7 @@ module normalization_lemmas {
             lemma_uint32_and_Q(b);
             assert c == 0;
             assert d == a0;
-            assert d == denormalize(uint16_as_nelem(a0));
+            assert d == MQN.denormalize(uint16_as_nelem(a0));
         }
         else {
             assert sa0 < 0;
@@ -110,7 +84,7 @@ module normalization_lemmas {
             lemma_uint32_and_Q(b);
             assert c == Q;
             assert d == sa0 + Q;
-            assert d == denormalize(uint16_as_nelem(a0));
+            assert d == MQN.denormalize(uint16_as_nelem(a0));
         }
     }
 
@@ -120,7 +94,8 @@ module normalization_lemmas {
     {
         && reveal normalized_values();
         && i <= N.full
-        && (forall j | 0 <= j < i :: dnv[j] == denormalize(uint16_as_nelem(nv[j])))
+        && (forall j | 0 <= j < i :: 
+            dnv[j] == MQN.denormalize(uint16_as_nelem(nv[j])))
     }
 
     lemma denormalization_pre_lemma(nv: seq<uint16>, dnv: seq<uint16>)
@@ -141,7 +116,7 @@ module normalization_lemmas {
         requires c == uint32_and(b, Q);
         requires d == uint32_add(a1, c);
         ensures uint16_is_normalized(buff[i]);
-        ensures d == denormalize(uint16_as_nelem(buff[i]));
+        ensures d == MQN.denormalize(uint16_as_nelem(buff[i]));
         ensures buff_is_n_elems(dnv[i := lh(d)]);
         ensures denormalization_inv(buff, dnv[i := lh(d)], i + 1);
     {
@@ -166,7 +141,7 @@ module normalization_lemmas {
         && inputs[i..] == outputs[i..]
         && (forall j | 0 <= j < i :: (
             && uint16_is_normalized(outputs[j])
-            && uint16_as_nelem(outputs[j]) == normalize(inputs[j]))
+            && uint16_as_nelem(outputs[j]) == MQN.normalize(inputs[j]))
         )
     }
 
@@ -200,7 +175,7 @@ module normalization_lemmas {
         if to_int32(b) >= 0 {
             assert d == 0;
             assume uh == 0; // the upper bits all clear
-            assert uint16_as_nelem(e) == normalize(a);
+            assert uint16_as_nelem(e) == MQN.normalize(a);
         } else {
             assert d == Q;
             assert 0 <= a < Q;
@@ -215,7 +190,7 @@ module normalization_lemmas {
             }
             assert bv16_op_s.to_int16(lh) == to_int32(e);
         }
-        assert uint16_as_nelem(lh) == normalize(a);
+        assert uint16_as_nelem(lh) == MQN.normalize(a);
     }
 
     lemma normalization_post_lemma(outputs: seq<uint16>, inputs: seq<uint16>)
@@ -227,20 +202,6 @@ module normalization_lemmas {
         reveal normalized_values();
     }
 
-    function l2norm_squared(s1: seq<nelem>, s2: seq<nelem>, i: nat): nat
-        requires |s1| == |s2|
-        requires i <= |s1|
-    {
-        if i == 0 then
-            0
-        else
-            var v1, v2 := s1[i-1] as int, s2[i-1] as int;
-            square_positive_lemma(v1);
-            square_positive_lemma(v2);
-            var vv1, vv2 := v1 * v1, v2 * v2;
-            l2norm_squared(s1, s2, i-1) + vv1 + vv2
-    }
-
     const NORMSQ_BOUND := integers.BASE_31
 
     predicate l2norm_squared_bounded_inv(norm: uint32, 
@@ -248,11 +209,11 @@ module normalization_lemmas {
     {
         && normalized_values(s1)
         && normalized_values(s2)
-        && var ns1 := uint16_buff_as_n_elems(s1);
-        && var ns2 := uint16_buff_as_n_elems(s2);
+        && var ns1 := uint16_buff_as_n_nelems(s1);
+        && var ns2 := uint16_buff_as_n_nelems(s2);
         && i <= N.full
-        && ((msb(ng) == 0) ==> (norm == l2norm_squared(ns1, ns2, i)))
-        && ((msb(ng) == 1) ==> (l2norm_squared(ns1, ns2, i) >= NORMSQ_BOUND))
+        && ((msb(ng) == 0) ==> (norm == MQN.l2norm_squared(ns1, ns2, i)))
+        && ((msb(ng) == 1) ==> (MQN.l2norm_squared(ns1, ns2, i) >= NORMSQ_BOUND))
     }
 
     lemma l2norm_squared_bounded_pre_lemma(s1: seq<uint16>, s2: seq<uint16>)
@@ -321,18 +282,18 @@ module normalization_lemmas {
         return; 
     }
 
-    predicate l2norm_squared_bounded(s1: seq<uint16>, s2: seq<uint16>)
-        requires normalized_values(s1);
-        requires normalized_values(s2);
+    predicate l2norm_squared_result(s1: seq<uint16>, s2: seq<uint16>, result: uint32)
     {
-        l2norm_squared(uint16_buff_as_n_elems(s1), uint16_buff_as_n_elems(s2), |s1|) < 0x29845d6
+        && normalized_values(s1)
+        && normalized_values(s2)
+        && ((result == 1) <==> (MQN.l2norm_squared(uint16_buff_as_n_nelems(s1), uint16_buff_as_n_nelems(s2), |s1|) < 0x29845d6))
     }
 
     lemma l2norm_squared_bounded_post_lemma(s1: seq<uint16>, s2: seq<uint16>, norm0: uint32, ng: uint32, norm1: uint32, result: uint32)
         requires l2norm_squared_bounded_inv(norm0, s1, s2, 512, ng);
         requires norm1 == uint32_or(norm0, uint32_srai(ng, 31));
         requires result == uint32_lt(norm1, 0x29845d6);
-        ensures (result == 1) <==> l2norm_squared_bounded(s1, s2)
+        ensures l2norm_squared_result(s1, s2, result);
     {
         if (msb(ng) == 0) {
             assume uint32_srai(ng, 31) == 0;
@@ -341,5 +302,27 @@ module normalization_lemmas {
             assume uint32_srai(ng, 31) == 0xffff_ffff;
             assume norm1 == 0xffff_ffff;
         }
+    }
+
+    lemma rv_falcon_512_lemma(tt0: seq<uint16>, tt1: seq<uint16>, tt2: seq<uint16>, s1: seq<uint16>, s2: seq<uint16>, h: seq<uint16>, c0: seq<uint16>, result: uint32)
+        requires l2norm_squared_result(s1, s2, result);
+        requires buff_is_n_elems(tt0);
+        requires buff_is_n_elems(c0);
+        requires buff_is_n_elems(h);
+        requires denormalization_inv(s2, tt0, 512);
+        requires tt1 == poly_mod_product(tt0, h);
+        requires poly_sub_loop_inv(tt2, tt1, c0, 512);
+        requires normalization_inv(s1, tt2, 512);
+        ensures (result == 1) <==> falcon_verify(c0, uint16_buff_as_n_nelems(s2), h);
+    {
+        reveal denormalization_inv();
+        assert tt0 == MQN.denormalize_n_elems(uint16_buff_as_n_nelems(s2));
+        assert tt1 == MQP.poly_mod(MQP.poly_mul(tt0, h), MQP.n_ideal());
+        assume c0 == buff_as_n_elems(c0);
+        assume h == buff_as_n_elems(h);
+        assert tt2 == MQP.poly_sub(tt1, c0);
+        reveal normalization_inv();
+        assert uint16_buff_as_n_nelems(s1) == MQN.normalize_elems(tt2);
+        assert falcon_512_i.bound() == 0x29845d6;
     }
 }
